executable_complete.v
@@ -9,6 +9,9 @@ Local Opaque singleton.
 Ltac solve_length := simplify_equality'; repeat
   match goal with H : Forall2 _ _ _ |- _ => apply Forall2_length in H end; lia.
 Hint Resolve cmap_refine_memenv_refine.
+Hint Immediate mem_inj_extend_reflexive.
+Hint Immediate ctx_typed_stack_typed.
+Hint Resolve (elem_of_singleton_2 (C:=listset (state Ti))).
 
 Lemma ehstep_exec_complete Γ Γf m1 m2 ρ τs e1 e2 τlr :
   ✓ Γ → ✓{Γ} m1 → '{m1} ⊢* ρ :* τs → (Γ,Γf,'{m1},τs) ⊢ e1 : τlr →
@@ -16,17 +19,11 @@ Lemma ehstep_exec_complete Γ Γf m1 m2 ρ τs e1 e2 τlr :
   (**i 1.) *) ehstep_exec Γ ρ e1 m1 = Some (e2', m2') ∧
   (**i 2.) *) e2' ⊑{(Γ,Γf,τs),f@'{m2'}↦'{m2}} e2 : τlr ∧
   (**i 3.) *) m2' ⊑{Γ,f} m2 ∧
-  (**i 4.) *) (∀ o τ, '{m1} ⊢ o : τ → '{m2} ⊢ o : τ) ∧
-  (**i 5.) *) (∀ o τ, '{m1} ⊢ o : τ → '{m2'} ⊢ o : τ) ∧
-  (**i 6.) *) (∀ o τ, '{m1} ⊢ o : τ → f !! o = Some (o,[])) ∧
-  (**i 7.) *) (∀ o τ,
-    '{m1} ⊢ o : τ → index_alive ('{m2'}) o → index_alive ('{m1}) o) ∧
-  (**i 8.) *) (∀ o o' r τ, '{m1} ⊢ o' : τ →
-    f !! o = Some (o',r) → mem_inj_id !! o = Some (o',r)).
+  (**i 4.) *) mem_inj_extend mem_inj_id f ('{m1}) ('{m1}).
 Proof.
   intros ? Hm1 Hρ He1 p. destruct (ehstep_preservation Γ Γf m1 m2 ρ
-    τs e1 e2 τlr) as (Hm2&He2&Hotyped&Hoalive); auto.
-  revert Hm1 Hρ He1 Hm2 He2 Hotyped Hoalive. case p; clear p; try by (
+    τs e1 e2 τlr) as (Hm2&He2&Hm); auto.
+  revert Hm1 Hρ He1 Hm2 He2 Hm. case p; clear p; try by (
     intros; repeat match goal with
     | H : assign_sem _ _ _ _ _ _ _ |- _ =>
        apply assign_exec_correct in H
@@ -34,24 +31,22 @@ Proof.
     | _ => progress simplify_option_equality
     end; eexists mem_inj_id, _, _; split_ands;
       eauto using cmap_refine_id', expr_refine_id).
-  intros m Ω o τi τ n ??????????; simplify_option_equality; typed_inversion_all.
+  intros m Ω o τi τ n ?????????; simplify_option_equality; typed_inversion_all.
   set (o' := fresh (dom indexset m)) in *.
   assert (mem_allocable o' m) by (apply mem_allocable_fresh).
   destruct (mem_alloc_refine' Γ mem_inj_id m m true (τ.[Z.to_nat n])
-    (fresh (dom indexset m)) o) as (f&?&?&?&?); auto using cmap_refine_id'.
+    (fresh (dom indexset m)) o) as (f&?&?&?); auto using cmap_refine_id'.
   eexists f, _, _; split_ands; eauto.
-  refine_constructor; eauto using lockset_valid_weaken, mem_alloc_index_typed.
+  refine_constructor; eauto using lockset_valid_weaken, mem_alloc_extend.
   * eapply locks_refine_weaken with mem_inj_id ('{m}) ('{m});
-      eauto using locks_refine_id,
-      mem_alloc_index_typed, mem_alloc_index_alive_inv, option_eq_1.
-  * eapply addr_top_array_refine; eauto using mem_alloc_index_typed_eq.
-  * eauto using mem_alloc_index_typed.
-  * eauto using mem_alloc_index_alive_inv.
+      eauto using locks_refine_id, mem_alloc_extend', option_eq_1.
+  * eapply addr_top_array_refine; eauto using mem_alloc_index_typed'.
 Qed.
-Hint Resolve (elem_of_singleton_2 (C:=listset (state Ti))).
 Lemma cstep_exec_complete Γ Γf δ S1 S2 g :
-  ✓ Γ → (Γ,'{SMem S1}) ⊢ δ : Γf → (Γ,Γf) ⊢ S1 : g → Γ\ δ ⊢ₛ S1 ⇒ S2 →
-  ∃ f S2', S2' ∈ cstep_exec Γ δ S1 ∧ S2' ⊑{(Γ,Γf),f} S2 : g.
+  ✓ Γ → (Γ,'{SMem S1}) ⊢ δ : Γf → (Γ,Γf) ⊢ S1 : g → Γ\ δ ⊢ₛ S1 ⇒ S2 → ∃ f S2',
+  (**i 1.) *) S2' ∈ cstep_exec Γ δ S1 ∧
+  (**i 2.) *) S2' ⊑{(Γ,Γf),f} S2 : g ∧
+  (**i 3.) *) mem_inj_extend mem_inj_id f ('{SMem S1}) ('{SMem S1}).
 Proof.
   intros ? Hδ1 HS1 p.
   destruct (cstep_preservation Γ Γf δ S1 S2 g) as [HS2 Hδ2]; auto.
@@ -62,22 +57,23 @@ Proof.
   * intros m k Ei e ????.
     eexists mem_inj_id, _; split_ands; eauto using state_refine_id.
     destruct Ei; simpl; eauto.
-  * intros m1 m2 k E e1 e2 ?? (τlr&Heτlr&?&?) _ _; simpl in *.
+  * intros m1 m2 k E e1 e2 ?? (τlr&Heτlr&?&?) ? _; simpl in *.
     typed_inversion Heτlr; edestruct (ectx_subst_typed_rev Γ Γf ('{m1})
       (get_stack_types k) E e1) as (τlr&?&?); eauto.
     edestruct (ehstep_exec_complete Γ Γf m1 m2 (get_stack k) (get_stack_types k)
-      e1 e2) as (f&e2'&m2'&?&?&?&?&?&?&?&?); eauto using ctx_typed_stack_typed.
-    exists f (State k (Expr (subst E e2')) m2'); split.
+      e1 e2) as (f&e2'&m2'&?&?&?&?); eauto using ctx_typed_stack_typed.
+    exists f (State k (Expr (subst E e2')) m2'); split_ands; auto.
     { assert (is_redex e1) as He1 by eauto using ehstep_is_redex.
       assert (maybe_EVal (subst E e1) = None) as ->.
       { destruct E as [|Ei] using rev_ind; [by destruct He1|].
         by destruct Ei; by rewrite ?subst_app. }
       apply elem_of_bind; exists (E, e1).
       simplify_option_equality; eauto using expr_redexes_complete. }
-    eexists; split_ands; repeat refine_constructor; eauto.
-    + eapply ectx_subst_refine; eauto.
-      eapply ectx_refine_weaken; eauto using ectx_refine_id.
-    + eapply ctx_refine_weaken; eauto using ctx_refine_id.
+    eleft; split_ands; repeat refine_constructor; eauto.
+    + eapply ectx_subst_refine; eauto 10 using ectx_refine_weaken,
+        ectx_refine_id, ehstep_extend, ehstep_exec_sound.
+    + eauto 10 using ctx_refine_weaken,
+        ctx_refine_id, ehstep_extend, ehstep_exec_sound.
   * intros m k f E Ωs vs ?????; simpl.
     eexists mem_inj_id, _; split_ands; eauto using state_refine_id.
     assert (maybe_EVal (subst E (call f @ #{Ωs}* vs)%E) = None) as ->.
@@ -103,21 +99,20 @@ Proof.
     edestruct (funenv_lookup Γ ('{m}) Γf δ h)
       as (?&?&?&?&?&?&?&?&?); eauto; simplify_equality'.
     edestruct (mem_alloc_val_list_refine' Γ mem_inj_id m m os' os vs vs) as
-      (f&?&?&?&?); eauto using cmap_refine_id', vals_refine_id.
+      (f&?&?&?); eauto using cmap_refine_id', vals_refine_id.
     exists f (State (CParams h (zip os' (type_of <$> vs)) :: k)
       (Stmt ↘ s) (mem_alloc_val_list Γ (zip os' vs) m)).
-    split; [unfold of_option; simplify_option_equality; esolve_elem_of|].
+    split_ands; auto.
+    { unfold of_option; simplify_option_equality; esolve_elem_of. }
     erewrite fmap_type_of by eauto.
-    eexists; split_ands; simpl; repeat refine_constructor;
-      eauto using mem_alloc_val_list_index_typed_eq.
+    eleft; split_ands; simpl; repeat refine_constructor;
+      eauto using mem_alloc_val_list_index_typed.
     + rewrite snd_zip by solve_length.
       erewrite Fun_type_stack_types, (right_id_L [] (++)) by eauto.
       eapply (stmt_refine_weaken _ _ mem_inj_id _ ('{m}));
-        eauto using stmt_refine_id, mem_alloc_val_list_index_typed,
-        mem_alloc_val_list_index_alive_inv.
+        eauto using stmt_refine_id, mem_alloc_val_list_extend.
     + eapply (ctx_refine_weaken _ _ mem_inj_id _ ('{m}));
-        eauto using ctx_refine_id, mem_alloc_val_list_index_typed,
-        mem_alloc_val_list_index_alive_inv.
+        eauto using ctx_refine_id, mem_alloc_val_list_extend.
   * intros m k l ????; simpl; rewrite decide_True by solve_elem_of.
     eexists mem_inj_id, _; split_ands; eauto using state_refine_id.
   * intros m k Es l s ?????; simpl.
@@ -130,19 +125,19 @@ Proof.
     assert (mem_allocable (fresh (dom indexset m)) m).
     { eapply mem_allocable_alt, is_fresh. }
     destruct (mem_alloc_refine' Γ mem_inj_id m m false τ
-      (fresh (dom indexset m)) o) as (f&?&?&?&?); auto using cmap_refine_id'.
+      (fresh (dom indexset m)) o) as (f&?&?&?); auto using cmap_refine_id'.
     eexists f, (State (CBlock (fresh (dom indexset m)) τ :: k) (Stmt d s)
       (mem_alloc Γ (fresh (dom indexset m)) false τ m)).
-    split; [by destruct d; simplify_option_equality; try case_match; eauto|].
-    eexists; split_ands; simpl; repeat refine_constructor;
-      eauto using mem_alloc_index_typed_eq.
-    + eapply (stmt_refine_weaken _ _ mem_inj_id _ ('{m})); eauto using
-        stmt_refine_id, mem_alloc_index_typed, mem_alloc_index_alive_inv.
+    split_ands; auto.
+    { by destruct d; simplify_option_equality; try case_match; eauto. }
+    eleft; split_ands; simpl; repeat refine_constructor;
+      eauto using mem_alloc_index_typed'.
+    + eapply (stmt_refine_weaken _ _ mem_inj_id _ ('{m}));
+        eauto using stmt_refine_id, mem_alloc_extend'.
     + eapply (direction_refine_weaken _ mem_inj_id _ ('{m})); eauto using
-        direction_refine_id, mem_alloc_index_typed,
-        mem_alloc_index_alive_inv, option_eq_1_alt.
-    + eapply (ctx_refine_weaken _ _ mem_inj_id _ ('{m})); eauto using
-        ctx_refine_id, mem_alloc_index_typed, mem_alloc_index_alive_inv.
+        direction_refine_id, mem_alloc_extend', option_eq_1_alt.
+    + eapply (ctx_refine_weaken _ _ mem_inj_id _ ('{m}));
+        eauto using ctx_refine_id, mem_alloc_extend'.
   * intros m k d o τ s ?????.
     eexists mem_inj_id, _; split_ands; eauto using state_refine_id.
     by destruct d; simpl; try case_match; eauto.
