permission_bits.v
@@ -85,8 +85,7 @@ Lemma pbits_valid_perm_valid Γ Γm xbs :
   ✓{Γ,Γm}* xbs → Forall sep_valid (tagged_perm <$> xbs).
 Proof. induction 1 as [|?? (?&?&?)]; csimpl; eauto. Qed.
 Lemma pbit_valid_weaken Γ1 Γ2 Γm1 Γm2 xb :
-  ✓ Γ1 → ✓{Γ1,Γm1} xb → Γ1 ⊆ Γ2 →
-  (∀ o τ, Γm1 ⊢ o : τ → Γm2 ⊢ o : τ) → ✓{Γ2,Γm2} xb.
+  ✓ Γ1 → ✓{Γ1,Γm1} xb → Γ1 ⊆ Γ2 → Γm1 ⊆{⇒} Γm2 → ✓{Γ2,Γm2} xb.
 Proof. intros ? (?&?&?); repeat split; eauto using bit_valid_weaken. Qed.
 Lemma pbit_valid_sep_valid Γ Γm xb  : ✓{Γ,Γm} xb → sep_valid xb.
 Proof. by intros (?&?&?); repeat split. Qed.
@@ -370,14 +369,9 @@ Global Instance:
   PropHolds (✓ Γ) → Transitive (refine Γ mem_inj_id Γm Γm : relation (pbit Ti)).
 Proof. intros Γ ?????. eapply @pbit_refine_compose; eauto; apply _. Qed.
 Lemma pbit_refine_weaken Γ Γ' f f' Γm1 Γm2 Γm1' Γm2' xb1 xb2 :
-  ✓ Γ → xb1 ⊑{Γ,f@Γm1↦Γm2} xb2 → Γ ⊆ Γ' → Γm1' ⊑{Γ',f'} Γm2' → 
-  (∀ o o2 r τ, Γm1 ⊢ o : τ → f !! o = Some (o2,r) → f' !! o = Some (o2,r)) →
-  (∀ o τ, Γm1 ⊢ o : τ → Γm1' ⊢ o : τ) → (∀ o τ, Γm2 ⊢ o : τ → Γm2' ⊢ o : τ) →
-  (∀ o τ, Γm1 ⊢ o : τ → index_alive Γm1' o → index_alive Γm1 o) →
-  xb1 ⊑{Γ',f'@Γm1'↦Γm2'} xb2.
-Proof.
-  intros ? (?&?&[??]&[??]); repeat split; eauto using bit_refine_weaken.
-Qed.
+  ✓ Γ → xb1 ⊑{Γ,f@Γm1↦Γm2} xb2 → Γ ⊆ Γ' → Γm1' ⊑{Γ',f'} Γm2' → Γm1 ⊆{⇒} Γm1' →
+  Γm2 ⊆{⇒} Γm2' → mem_inj_extend f f' Γm1 Γm2 → xb1 ⊑{Γ',f'@Γm1'↦Γm2'} xb2.
+Proof. intros ? (?&?&[]&[]); repeat split; eauto using bit_refine_weaken. Qed.
 Lemma pbits_refine_perm Γ f Γm1 Γm2 xbs1 xbs2 :
   xbs1 ⊑{Γ,f@Γm1↦Γm2}* xbs2 → tagged_perm <$> xbs1 = tagged_perm <$> xbs2.
 Proof. induction 1 as [|???? (?&?&?&?)]; f_equal'; auto. Qed.
