type_preservation.v
@@ -44,9 +44,7 @@ Lemma ehstep_preservation Γ Γf m1 m2 ρ τs e1 e2 τlr :
   ✓{Γ} m1 → (Γ,Γf,'{m1},τs) ⊢ e1 : τlr → '{m1} ⊢* ρ :* τs →
   (**i 1.) *) ✓{Γ} m2 ∧
   (**i 2.) *) (Γ,Γf,'{m2},τs) ⊢ e2 : τlr ∧
-  (**i 3.) *) (∀ o τ, '{m1} ⊢ o : τ → '{m2} ⊢ o : τ) ∧
-  (**i 4.) *) (∀ o τ,
-    '{m1} ⊢ o : τ → index_alive ('{m2}) o → index_alive ('{m1}) o).
+  (**i 3.) *) '{m1} ⊆{⇒} '{m2}.
 Proof.
   intros ? [] ???.
   * typed_inversion_all; decompose_Forall_hyps; split_ands; auto.
@@ -55,36 +53,33 @@ Proof.
   * typed_inversion_all; auto.
   * typed_inversion_all; auto 7.
   * typed_inversion_all.
-    rewrite <-!and_assoc; split; [apply and_wlog_l; intros; split_ands|].
+    rewrite <-and_assoc; apply and_wlog_l; intros; split_ands.
     + eapply mem_lock_valid'; eauto using mem_insert_writable,
         mem_insert_valid', assign_preservation_2.
     + typed_constructor; eauto using lockset_union_valid, lockset_valid_weaken,
         lock_singleton_valid, val_typed_weaken, assign_preservation_1.
-    + intros. eapply mem_lock_index_typed; eauto using mem_insert_writable,
-        mem_insert_valid', mem_insert_index_typed, assign_preservation_2.
-    + intros ???. by erewrite mem_lock_memenv_of, mem_insert_memenv_of
-        by eauto using mem_insert_writable,
+    + intros. erewrite mem_lock_memenv_of by eauto using mem_insert_writable,
         mem_insert_valid', assign_preservation_2.
-  * typed_inversion_all; split_ands.
+      eauto using mem_insert_extend, assign_preservation_2.
+  * typed_inversion_all.
+    rewrite <-and_assoc; apply and_wlog_l; intros; split_ands.
     + eauto using mem_force_valid'.
-    + typed_constructor; eauto using lockset_valid_weaken, mem_force_index_typed.
-      eauto 6 using val_typed_weaken, mem_force_index_typed, mem_lookup_typed.
-    + eauto using mem_lookup_typed, mem_force_index_typed.
-    + intros ???. by erewrite mem_force_memenv_of by eauto.
+    + typed_constructor; eauto using lockset_valid_weaken,
+        val_typed_weaken,  mem_lookup_typed.
+    + eauto using mem_lookup_typed, mem_force_extend.
   * typed_inversion_all.
     split_ands; eauto 7 using addr_elt_typed, addr_elt_strict.
   * typed_inversion_all; split_ands; eauto using val_lookup_seg_typed.
   * typed_inversion_all.
-    rewrite <-!and_assoc; split; [apply and_wlog_l; intros; split_ands|].
+    rewrite <-and_assoc; apply and_wlog_l; intros; split_ands.
     + eapply mem_alloc_valid'; eauto using TArray_valid.
       by rewrite size_of_array, Nat2Z.inj_mul, Z2Nat.id
         by auto using Z_to_nat_neq_0_nonneg.
     + typed_constructor; eauto using addr_top_array_strict, TArray_valid,
-        addr_top_array_typed, mem_alloc_index_typed_eq, lockset_valid_weaken.
-    + eauto using mem_alloc_index_typed, TArray_valid.
-    + eauto using mem_alloc_index_alive_inv, TArray_valid.
-  * typed_inversion_all; split_ands; eauto 10 using lockset_valid_weaken,
-      mem_free_valid', mem_free_index_typed, mem_free_index_alive_inv.
+        addr_top_array_typed, mem_alloc_index_typed', lockset_valid_weaken.
+    + eauto using mem_alloc_extend', TArray_valid.
+  * typed_inversion_all; split_ands; eauto using
+      lockset_valid_weaken, mem_free_valid', mem_free_extend'.
   * typed_inversion_all;
       repeat match goal with H : unop_typed _ _ _ |- _ => by inversion H end;
       split_ands; eauto using val_unop_typed.
@@ -92,18 +87,22 @@ Proof.
       repeat match goal with H : binop_typed _ _ _ _ |- _ => by inversion H end;
       split_ands; eauto using val_binop_typed, lockset_union_valid.
   * typed_inversion_all; split_ands; eauto using mem_unlock_valid',
-      expr_typed_weaken, mem_unlock_index_typed, mem_unlock_index_alive_inv.
+      expr_typed_weaken, mem_unlock_extend.
   * typed_inversion_all; split_ands; eauto using mem_unlock_valid',
-      expr_typed_weaken, mem_unlock_index_typed, mem_unlock_index_alive_inv.
+      expr_typed_weaken, mem_unlock_extend.
   * typed_inversion_all; split_ands; eauto using mem_unlock_valid',
-      expr_typed_weaken, mem_unlock_index_typed, mem_unlock_index_alive_inv.
+      expr_typed_weaken, mem_unlock_extend.
   * typed_inversion_all;
       repeat match goal with H : cast_typed _ _ _ |- _ => by inversion H end;
       split_ands; eauto using val_cast_typed.
 Qed.
+Lemma ehstep_extend Γ Γf m1 m2 ρ τs e1 e2 τlr :
+  ✓ Γ → Γ\ ρ ⊢ₕ e1, m1 ⇒ e2, m2 → ✓{Γ} m1 → (Γ,Γf,'{m1},τs) ⊢ e1 : τlr →
+  '{m1} ⊢* ρ :* τs → '{m1} ⊆{⇒} '{m2}.
+Proof. intros. eapply ehstep_preservation; eauto. Qed.
 Lemma cstep_preservation Γ Γf δ S1 S2 f :
   ✓ Γ → Γ\ δ ⊢ₛ S1 ⇒ S2 → (Γ,Γf) ⊢ S1 : f → (Γ,'{SMem S1}) ⊢ δ : Γf →
-  (Γ,Γf) ⊢ S2 : f ∧ (Γ,'{SMem S2}) ⊢ δ : Γf.
+  (Γ,Γf) ⊢ S2 : f ∧ '{SMem S1} ⊆{⇒} '{SMem S2}.
 Proof.
   intros ? p. case p; clear p.
   * intros m k (τf&HS&?&?) ?; typed_inversion_all; split; auto.
@@ -117,7 +116,7 @@ Proof.
     edestruct (ectx_subst_typed_rev Γ Γf ('{m1})
       (get_stack_types k) E e1) as (τrl&?&?); eauto.
     destruct (ehstep_preservation Γ Γf m1 m2 (get_stack k) (get_stack_types k)
-      e1 e2 τrl) as (?&?&?&_); eauto using ctx_typed_stack_typed.
+      e1 e2 τrl) as (?&?&?); eauto using ctx_typed_stack_typed.
     split; [|eauto using funenv_typed_weaken].
     eexists; simpl; split_ands; eauto using ctx_typed_weaken,
       ectx_subst_typed, ectx_typed_weaken.
@@ -125,59 +124,59 @@ Proof.
     edestruct (ectx_subst_typed_rev Γ Γf ('{m})
       (get_stack_types k) E (call f' @ #{Ωs}* vs)) as (τrl&Hcall&?); eauto.
     typed_inversion Hcall.
-    split; [|eauto using funenv_typed_weaken, mem_unlock_index_typed].
+    split; [|eauto using funenv_typed_weaken, mem_unlock_extend].
     eexists (Fun_type f'); simpl; split_ands; eauto using mem_unlock_valid'.
     + typed_constructor; eauto.
       eapply (EVals_typed_inv Γ Γf _ (get_stack_types k));
         eauto using funenv_typed_funtypes_valid, funtypes_valid_args_valid,
-        Forall2_impl, expr_typed_weaken, mem_unlock_index_typed.
-    + repeat typed_constructor; eauto using ectx_typed_weaken,
-        ctx_typed_weaken, mem_unlock_index_typed.
+        Forall2_impl, expr_typed_weaken, mem_unlock_extend.
+    + repeat typed_constructor;
+        eauto using ectx_typed_weaken, ctx_typed_weaken, mem_unlock_extend.
   * intros m k E e ?? (τf&HS&?&?) ?; typed_inversion HS; split; auto.
     edestruct (ectx_subst_typed_rev Γ Γf ('{m})
       (get_stack_types k) E e) as (τrl&?&?); eauto.
   * intros m k e Ω v (τf&HS&?&?) ?; typed_inversion HS.
-    split; [|eauto using funenv_typed_weaken, mem_unlock_index_typed].
+    split; [|eauto using funenv_typed_weaken, mem_unlock_extend].
     typed_inversion_all.
     eexists; simpl; split_ands; repeat typed_constructor;
-      eauto using ctx_typed_weaken, mem_unlock_index_typed,
+      eauto using ctx_typed_weaken, mem_unlock_extend,
       mem_unlock_valid', expr_typed_weaken.
   * intros m k e Ω v (τf&HS&?&?) ?; typed_inversion HS.
-    split; [|eauto using funenv_typed_weaken, mem_unlock_index_typed].
+    split; [|eauto using funenv_typed_weaken, mem_unlock_extend].
     typed_inversion_all.
     eexists; simpl; split_ands; repeat typed_constructor;
-      eauto using ctx_typed_weaken, mem_unlock_index_typed, val_typed_weaken,
+      eauto using ctx_typed_weaken, mem_unlock_extend, val_typed_weaken,
       mem_unlock_valid', expr_typed_weaken.
   * intros m k e Ω v s ?  (τf&HS&?&?) ?; typed_inversion_all.
-    split; [|eauto using funenv_typed_weaken, mem_unlock_index_typed].
+    split; [|eauto using funenv_typed_weaken, mem_unlock_extend].
     eexists; simpl; split_ands; repeat typed_constructor;
       eauto using ctx_typed_weaken, expr_typed_weaken,
-      stmt_typed_weaken, mem_unlock_index_typed, mem_unlock_valid'.
+      stmt_typed_weaken, mem_unlock_extend, mem_unlock_valid'.
   * intros m k e Ω v s ?  (τf&HS&?&?) ?; typed_inversion_all.
-    split; [|eauto using funenv_typed_weaken, mem_unlock_index_typed].
+    split; [|eauto using funenv_typed_weaken, mem_unlock_extend].
     eexists; simpl; split_ands; repeat typed_constructor;
       eauto using ctx_typed_weaken, expr_typed_weaken,
-      stmt_typed_weaken, mem_unlock_index_typed, mem_unlock_valid'.
+      stmt_typed_weaken, mem_unlock_extend, mem_unlock_valid'.
   * intros m k e Ω v s ?? (τf&HS&?&?) ?; typed_inversion_all.
-    split; [|eauto using funenv_typed_weaken, mem_unlock_index_typed].
+    split; [|eauto using funenv_typed_weaken, mem_unlock_extend].
     eexists; simpl; split_ands; repeat typed_constructor;
       eauto using ctx_typed_weaken, expr_typed_weaken,
-      stmt_typed_weaken, mem_unlock_index_typed, mem_unlock_valid.
+      stmt_typed_weaken, mem_unlock_extend, mem_unlock_valid.
   * intros m k e Ω v s1 s2 ? (τf&HS&?&?) ?; typed_inversion_all.
-    split; [|eauto using funenv_typed_weaken, mem_unlock_index_typed].
+    split; [|eauto using funenv_typed_weaken, mem_unlock_extend].
     eexists; simpl; split_ands; repeat typed_constructor;
       eauto using ctx_typed_weaken, expr_typed_weaken,
-      stmt_typed_weaken, mem_unlock_index_typed, mem_unlock_valid'.
+      stmt_typed_weaken, mem_unlock_extend, mem_unlock_valid'.
   * intros m k e Ω v s1 s2 ? (τf&HS&?&?) ?; typed_inversion_all.
-    split; [|eauto using funenv_typed_weaken, mem_unlock_index_typed].
+    split; [|eauto using funenv_typed_weaken, mem_unlock_extend].
     eexists; simpl; split_ands; repeat typed_constructor;
       eauto using ctx_typed_weaken, expr_typed_weaken,
-      stmt_typed_weaken, mem_unlock_index_typed, mem_unlock_valid'.
+      stmt_typed_weaken, mem_unlock_extend, mem_unlock_valid'.
   * intros m k e Ω v s1 s2 ?? (τf&HS&?&?) ?; typed_inversion_all.
-    split; [|eauto using funenv_typed_weaken, mem_unlock_index_typed].
+    split; [|eauto using funenv_typed_weaken, mem_unlock_extend].
     eexists; simpl; split_ands; repeat typed_constructor;
       eauto using ctx_typed_weaken, expr_typed_weaken,
-      stmt_typed_weaken, mem_unlock_index_typed, mem_unlock_valid.
+      stmt_typed_weaken, mem_unlock_extend, mem_unlock_valid.
   * intros m k s1 s2 (τf&HS&?&?) ?; typed_inversion_all; split; auto.
     eexists; simpl; split_ands; eauto; repeat typed_constructor; eauto.
   * intros m k s1 s2 (τf&HS&?&?) ?; typed_inversion_all; split; auto.
@@ -195,7 +194,7 @@ Proof.
     edestruct (funenv_lookup Γ ('{m}) Γf δ f')
       as (s'&mτ&?&?&?&?&?&?&?); eauto.
     erewrite fmap_type_of by eauto; simplify_equality.
-    edestruct (mem_alloc_val_list_valid Γ m) as (?&?&?&?); eauto.
+    edestruct (mem_alloc_val_list_valid Γ m) as (?&?&?); eauto.
     split; [|eauto using funenv_typed_weaken].
     eexists; simpl; split_ands;
       repeat typed_constructor; eauto using ctx_typed_weaken.
@@ -203,16 +202,15 @@ Proof.
     rewrite snd_zip by (erewrite <-Forall2_length by eauto; lia).
     eauto using stmt_typed_weaken.
   * intros m k g oσs s (τf&HS&?&?) ?. typed_inversion_all.
-    split; [|eauto using funenv_typed_weaken, mem_foldr_free_index_typed].
+    split; [|eauto using funenv_typed_weaken, mem_foldr_free_extend].
     case_match; simplify_equality; try done.
-    eexists; simpl; split_ands; repeat typed_constructor;
-      eauto using ctx_typed_weaken, mem_foldr_free_index_typed,
-      mem_foldr_free_valid.
+    eexists; simpl; split_ands; repeat typed_constructor; eauto using
+      ctx_typed_weaken, mem_foldr_free_extend, mem_foldr_free_valid.
   * intros m k g oσs v s (τf&HS&?&?) ?; typed_inversion_all.
-    split; [|eauto using funenv_typed_weaken, mem_foldr_free_index_typed].
+    split; [|eauto using funenv_typed_weaken, mem_foldr_free_extend].
     case_match; simplify_equality; try done.
     eexists; simpl; split_ands; repeat typed_constructor;
-      eauto using ctx_typed_weaken, mem_foldr_free_index_typed,
+      eauto using ctx_typed_weaken, mem_foldr_free_extend,
       mem_foldr_free_valid, val_typed_weaken.
   * intros m k g E v (τf&HS&?&?) ?; typed_inversion_all; split; auto.
     eexists; simpl; split_ands; repeat typed_constructor;
@@ -231,25 +229,30 @@ Proof.
     eexists; simpl; split_ands; repeat typed_constructor;
       eauto using sctx_item_subst_typed.
   * intros m k d o τ s ?? (τf&HS&?&?) ?; typed_inversion_all.
-    split; [|eauto using funenv_typed_weaken, mem_alloc_index_typed].
-    eexists; simpl; split_ands; eauto 6 using mem_alloc_valid',
-      mem_alloc_index_typed, stmt_typed_weaken,
-      direction_typed_weaken, ctx_typed_weaken, mem_alloc_index_typed_eq.
+    split; [|eauto using funenv_typed_weaken, mem_alloc_extend'].
+    eexists; simpl; split_ands; eauto 6 using
+      mem_alloc_valid', stmt_typed_weaken, mem_alloc_extend',
+      direction_typed_weaken, ctx_typed_weaken, mem_alloc_index_typed'.
   * intros m k d o τ s ? (τf&HS&?&?) ?; typed_inversion_all.
-    split; [|eauto using funenv_typed_weaken, mem_free_index_typed].
-    eexists; simpl; split_ands; repeat typed_constructor;
-      eauto using ctx_typed_weaken, direction_typed_weaken,
-      mem_free_index_typed,
+    split; [|eauto using funenv_typed_weaken, mem_free_extend'].
+    eexists; simpl; split_ands; repeat typed_constructor; eauto using
+      ctx_typed_weaken, direction_typed_weaken, mem_free_extend',
       mem_free_valid', index_typed_valid, index_typed_representable.
-    eapply stmt_typed_weaken; eauto using mem_free_index_typed.
+    eapply stmt_typed_weaken; eauto using mem_free_extend'.
 Qed.
 Lemma csteps_preservation Γ Γf δ S1 S2 f :
   ✓ Γ → Γ\ δ ⊢ₛ S1 ⇒* S2 → (Γ,Γf) ⊢ S1 : f → (Γ,'{SMem S1}) ⊢ δ : Γf →
-  (Γ,Γf) ⊢ S2 : f ∧ (Γ,'{SMem S2}) ⊢ δ : Γf.
+  (Γ,Γf) ⊢ S2 : f ∧ '{SMem S1} ⊆{⇒} '{SMem S2}.
 Proof.
-  induction 2 as [|S1 S2 S3]; intros; [done|].
-  destruct (cstep_preservation Γ Γf δ S1 S2 f); auto.
+  induction 2 as [|S1 S2 S3 ?? IH]; intros; [done|].
+  destruct (cstep_preservation Γ Γf δ S1 S2 f) as (?&?); auto.
+  destruct IH as (?&?); split_ands; eauto using funenv_typed_weaken.
+  etransitivity; eauto.
 Qed.
+Lemma csteps_extend Γ Γf δ S1 S2 f :
+  ✓ Γ → Γ\ δ ⊢ₛ S1 ⇒* S2 → (Γ,Γf) ⊢ S1 : f → (Γ,'{SMem S1}) ⊢ δ : Γf →
+  '{SMem S1} ⊆{⇒} '{SMem S2}.
+Proof. intros. eapply csteps_preservation; eauto. Qed.
 
 Ltac ctx_inversion Hk :=
   typed_inversion Hk;
@@ -307,7 +310,8 @@ Lemma csteps_initial_progress Γ Γf δ m f vs S σs σ :
   (**i 3.) *) is_undef_state S.
 Proof.
   intros. assert ((Γ,Γf) ⊢ S : f ∧ (Γ,'{SMem S}) ⊢ δ : Γf) as [??].
-  { eauto using csteps_preservation, initial_state_typed. }
+  { destruct (csteps_preservation Γ Γf δ (initial_state m f vs) S f);
+      eauto using initial_state_typed, funenv_typed_weaken. }
   destruct (cstep_progress Γ Γf δ S f) as [?|[[v ?]|[?|(l&s&?&[])]]]; eauto.
   destruct S as [k φ m2]; simplify_equality'.
   eauto using csteps_initial_gotos, funenv_lookup_gotos.
